$$
y - y_1 = m(x - x_1)
$$

where:
- \( m \) is the slope of the line, given by the [Slope Equation](obsidian://open?vault=Documentation&file=Formulas%2FSlope%2FSlope),
- \( (x_1, y_1) \) is a known point on the line.

### How to Solve for \( y \) (Convert to Slope-Intercept Form):
1. **Substitute the given values** for \( x_1 \), \( y_1 \), and \( m \) into the equation.
2. **Distribute** \( m \) to both terms inside the parentheses.
3. **Isolate \( y \)** by adding \( y_1 \) to both sides to get the equation in slope-intercept form (\( y = mx + b \)).

### Example Calculation:
#### Given:
- \( m = 3 \)
- \( (x_1, y_1) = (2, 5) \)

#### Step 1: Plug in the values
$$
y - 5 = 3(x - 2)
$$

#### Step 2: Distribute \( m = 3 \)
$$
y - 5 = 3x - 6
$$

#### Step 3: Isolate \( y \)
$$
y = 3x - 6 + 5
$$
$$
y = 3x - 1
$$

This is the equation of the line in **slope-intercept form**.

Let me know if you need any refinements! ðŸš€
